theories/interop/wp_prims/read_foreign.v
@@ -4,7 +4,7 @@ From melocoton Require Import named_props stdpp_extra.
 From melocoton.mlanguage Require Import mlanguage.
 From melocoton.c_interface Require Import defs notation resources.
 From melocoton.interop Require Import state lang basics_resources.
-From melocoton.interop Require Export prims weakestpre prims_proto.
+From melocoton.interop Require Export prims weakestpre prims_proto update_laws.
 From melocoton.interop.wp_prims Require Import common.
 From melocoton.mlanguage Require Import weakestpre.
 Import Wrap.
@@ -28,13 +28,11 @@ Proof using.
   rewrite weakestpre.wp_unfold. rewrite /weakestpre.wp_pre.
   iIntros "%σ Hσ". cbn -[wrap_prog].
   SI_at_boundary. iNamed "HGC". SI_GC_agree.
-  iAssert ⌜ζC ρc !! γ = Some (Bforeign m (Some w'))⌝%I as "%Helem2".
+  iAssert ⌜∃ m', ζC ρc !! γ = Some (Bforeign m' (Some w'))⌝%I as "%Helem2".
   {
-    iDestruct (hgh_lookup_block with "GCHGH Hpto") as %(b&Hb&Hγ).
-    inversion Hb; subst; eauto.
-    iPureIntro. (* contradiction with Hγ *)
-    admit.
+    iDestruct (hgh_lookup_foreign with "GCHGH Hpto") as %(?&_&?). iPureIntro. eauto.
   }
+  destruct Helem2 as [m' Helem2].
   iApply wp_pre_cases_c_prim; [done..|].
   iExists (λ '(e', σ'), e' = WrSE (ExprV w') ∧ σ' = CState ρc mem).
   iSplit. { iPureIntro; econstructor; eauto. }
@@ -45,6 +43,6 @@ Proof using.
   iApply ("Cont" with "[- $Hpto]").
   rewrite /GC /named. iExists _, _, σMLvirt, _, _.
   iFrame. iPureIntro; split_and!; eauto.
-Admitted.
+Qed.
 
 End Laws.
